\begin{problem}{3}
Considera que:
\begin{align*}
\mathbf{\Sigma} &=
\begin{bmatrix}
10&-3&-1&5\\
-3&8&3&0\\
-1&3&15&1\\
5&0&1&4
\end{bmatrix}
\end{align*}
Obtener A) Cov$(2X_1,-4X_2)$. B) Var$(3X_2-2X_3)$. C)Var$(2X_1-4X_2+3X_3-X_4)$
\end{problem}

\begin{sol}
\begin{itemize}
\item A) Cov$(2X_1,-4X_2)$\\
Usando la propiedad Cov$(aX_1,bX_2)=ab \sigma_{12}$, donde $\sigma_{12}$ la encontramos en $\mathbf{\Sigma}$ como $\sigma_{12}=-3$.
\begin{align*}
\text{Cov}(2X_1,-4X_2) &= 2 \cdot -4 \cdot -3 \\
\text{Cov}(2X_1,-4X_2) &=  24
\end{align*}

\item B) Var$(3X_2-2X_3)$ \\
Usando la propiedad Var$(aX_1+bX_2)=a^2\sigma_{11}+b^2\sigma_{22}+2ab\sigma_{12}$ encontramos en $\mathbf{\Sigma}$
lo siguiente: $\sigma_{22}=8,\sigma_{33}=15,\sigma_{23}=3$.
\begin{align*}
\text{Var}(3X_2-2X_3) &= 3^2 \cdot 8 + (-2)^2 \cdot 15 + 2 \cdot 3 \cdot (-2) \cdot 3\\
\text{Var}(3X_2-2X_3) &= 72+60-36\\
\text{Var}(3X_2-2X_3) &= 96\\
\end{align*}
\item C) Var$(2X_1-4X_2+3X_3-X_4)$ \\
La combinación lineal está dada por:
\begin{align*}
\mathbf{X}= \begin{pmatrix}
X_1\\X_2\\X_3\\X_4
\end{pmatrix},
\mathbf{c} = \begin{pmatrix}
2\\-4\\3\\-1
\end{pmatrix}
\end{align*}
Usando la propiedad: Var$(\mathbf{c'X})=\mathbf{c' \Sigma c}$ tenemos:
\begin{align*}
\mathbf{c' \Sigma c} &=
\begin{pmatrix}
2 & -4 & 3 & -1 
\end{pmatrix}
\begin{pmatrix}
10&-3&-1&5\\
-3&8&3&0\\
-1&3&15&1\\
5&0&1&4
\end{pmatrix}
\begin{pmatrix}
2 \\ -4 \\ 3 \\ -1 
\end{pmatrix}\\
&= \begin{pmatrix}
20 + 12 -3-5& -6-32+9+0 & -2-12+45-1 & 10+0+3 -4 
\end{pmatrix}
\begin{pmatrix}
2 \\ -4 \\ 3 \\ -1 
\end{pmatrix}\\
&= \begin{pmatrix}
24& -29& 30 & 9
\end{pmatrix}
\begin{pmatrix}
2 \\ -4 \\ 3 \\ -1 
\end{pmatrix}=
\begin{pmatrix}
(24)(2)+(-29)(-4)+(30)(3)+(9)(-1)\\
\end{pmatrix}
=
\begin{pmatrix}
116+90-9
\end{pmatrix}\\
& \therefore \text{Var}(2X_1-4X_2+3X_3-X_4)=245
\end{align*}

\end{itemize}
\end{sol}